theories/Type/WellFounded.v
@@ -1,7 +1,7 @@
 Set Warnings "-notation-overridden".
 From Coq Require Import Extraction CRelationClasses.
 Require Import Equations.Init Equations.Tactics.
-Require Import Equations.Type.Logic
+Require Import Equations.Type.Logic Equations.Type.FunctionalExtensionality
         Equations.Type.Relation Equations.Type.Relation_Properties.
 
 Set Universe Polymorphism.
@@ -10,7 +10,7 @@ Import Sigma_Notations.
 
 (** Well-founded relations in Type *)
 
-Section Wf.
+Section Acc.
 
   Context {A} (R : relation A).
 
@@ -20,9 +20,50 @@ Section Wf.
   Definition Acc_inv {x} (H : Acc x) : forall y, R y x -> Acc y.
   Proof. intros y Hy. destruct H. exact (a _ Hy). Defined.
 
+  Lemma Acc_prop i (x y : Acc i) : x = y.
+  Proof.
+    revert y.
+    induction x as [y Accy IHy].
+    intros [Accy']. apply ap.
+    apply funext. intros H.
+    apply funext. intros H'.
+    apply IHy.
+  Qed.
+
   Definition well_founded := forall x, Acc x.
 
-End Wf.
+  Context (P : A -> Type).
+  Context (step : forall x : A, (forall y : A, R y x -> P y) -> P x).
+
+  Fixpoint Fix_F (x : A) (a : Acc x) : P x :=
+    step x (fun y r => Fix_F y (Acc_inv a y r)).
+
+End Acc.
+
+Section FixWf.
+  Context {A R} (WF : @well_founded A R).
+  Context (P : A -> Type).
+  Context (step : forall x : A, (forall y : A, R y x -> P y) -> P x).
+
+  Definition Fix (x : A) : P x :=
+    Fix_F R P step x (WF x).
+End FixWf.
+
+Lemma well_founded_irreflexive {A} {R : relation A} {wfR : well_founded R} :
+  forall x y : A, R x y -> x = y -> Empty.
+Proof.
+  intros x y Ryy. intros e. destruct e. red in wfR.
+  induction (wfR x) as [y accy IHy].
+  apply (IHy _ Ryy Ryy).
+Qed.
+
+Lemma well_founded_antisym@{i j} {A : Type@{i}} {R : relation@{i j} A}{wfR : well_founded R} :
+  forall x y : A, R x y -> R y x -> Empty.
+Proof.
+  intros x y Rxy Ryx. red in wfR.
+  induction (wfR y) as [y accy IHy] in x, Rxy, Ryx.
+  specialize (IHy _ Rxy). apply (IHy _ Ryx Rxy).
+Qed.
 
 Section Wf_Transitive_Closure.
 
@@ -58,10 +99,51 @@ Section Wf_Transitive_Closure.
 
 End Wf_Transitive_Closure.
 
-Lemma well_founded_irreflexive {A} {R : relation A} {wfR : well_founded R} :
-  forall x y : A, R x y -> x = y -> Empty.
-Proof.
-  intros x y Ryy. intros e. destruct e. red in wfR.
-  induction (wfR x) as [y accy IHy].
-  apply (IHy _ Ryy Ryy).
-Qed.
+(** Author: Bruno Barras *)
+
+Section Inverse_Image.
+
+  Context {A B : Type} (R : relation B) (f : A -> B).
+
+  Definition inverse_image := fun x y => R (f x) (f y).
+
+  Remark Acc_lemma : forall y : B, Acc R y -> forall x : A, y = f x -> Acc inverse_image x.
+  Proof.
+    induction 1 as [y _ IHAcc]; intros x H.
+    apply Acc_intro; intros y0 H1.
+    apply (IHAcc (f y0)); try trivial.
+    apply id_sym in H. destruct H; trivial. constructor.
+  Defined.
+
+  Lemma Acc_inverse_image : forall x:A, Acc R (f x) -> Acc inverse_image x.
+  Proof.
+    intros; apply (Acc_lemma (f x)); trivial. constructor.
+  Defined.
+
+  Theorem wf_inverse_image : well_founded R -> well_founded inverse_image.
+  Proof.
+    red; intros; apply Acc_inverse_image; auto.
+  Defined.
+
+  (* Variable F : A -> B -> Type. *)
+  (* Let RoF (x y:A) := *)
+  (*   exists2 b : B, F x b & (forall c:B, F y c -> R b c). *)
+
+  (* Lemma Acc_inverse_rel : forall b:B, Acc R b -> forall x:A, F x b -> Acc RoF x. *)
+  (* Proof. *)
+  (*   induction 1 as [x _ IHAcc]; intros x0 H2. *)
+  (*   constructor; intros y H3. *)
+  (*   destruct H3. *)
+  (*   apply (IHAcc x1); auto. *)
+  (* Qed. *)
+
+
+  (* Theorem wf_inverse_rel : well_founded R -> well_founded RoF. *)
+  (* Proof. *)
+  (*   red; constructor; intros. *)
+  (*   case H0; intros. *)
+  (*   apply (Acc_inverse_rel x); auto. *)
+  (* Qed. *)
+
+End Inverse_Image.
+
