examples/ordinal_rec.v
@@ -2,7 +2,7 @@ From Equations Require Import Equations Fin.
 (* Add LoadPath "examples". *)
 Require Import ordinals.
 Add Search Blacklist "_obligation_".
-From Equations Require Import TransparentEquations.
+Require Import Equations.Prop.TransparentEquations.
 
 Inductive ho : Set :=
 | base : nat -> ho
