theories/Prop/Telescopes.v
@@ -1,5 +1,5 @@
 Require Import Equations.Prop.Loader.
-Require Import FunctionalExtensionality.
+From Coq Require Import FunctionalExtensionality.
 Require Import Equations.Prop.DepElim.
 (** Telescopes: allows treating variable arity fixpoints *)
 Set Universe Polymorphism.
